- finished generate proof - renamed hmac_drbg_update_post - style changes

specs/HMAC_DRBG_generate_algorithm.v
@@ -24,7 +24,7 @@ Proof.
 Defined.
 
 Function HMAC_DRBG_generate_helper_Z (HMAC: list Z -> list Z -> list Z) (key v: list Z) (requested_number_of_bytes: Z) {measure Z.to_nat requested_number_of_bytes}: (list Z * list Z) :=
-  if Z.geb 0 requested_number_of_bytes then (v, [])
+  if (0 >=? requested_number_of_bytes) then (v, [])
   else
     let len := 32%nat in (* TODO get this from property of HMAC *)
     let (v, rest) := HMAC_DRBG_generate_helper_Z HMAC key v (requested_number_of_bytes - (Z.of_nat len)) in
@@ -410,15 +410,16 @@ Proof.
 Qed.
 
 Definition HMAC_DRBG_generate_algorithm (HMAC: list Z -> list Z -> list Z) (reseed_interval: Z) (working_state: DRBG_working_state) (requested_number_of_bytes: Z) (additional_input: list Z): DRBG_generate_algorithm_result :=
-  let '(v, key, reseed_counter) := working_state in
-  if Z.gtb reseed_counter reseed_interval then generate_algorithm_reseed_required
-  else
-    let (key, v) := match additional_input with
-                      | [] => (key, v)
-                      | _::_ => HMAC_DRBG_update HMAC additional_input key v
-                    end in
-    let (v, temp) := HMAC_DRBG_generate_helper_Z HMAC key v requested_number_of_bytes in
-    let returned_bits := firstn (Z.to_nat requested_number_of_bytes) temp in
-    let (key, v) := HMAC_DRBG_update HMAC additional_input key v in
-    let reseed_counter := reseed_counter + 1 in
-    generate_algorithm_success returned_bits (v, key, reseed_counter).      
+  match working_state with (v, key, reseed_counter) =>
+    if Z.gtb reseed_counter reseed_interval then generate_algorithm_reseed_required
+    else
+      let (key, v) := match additional_input with
+                        | [] => (key, v)
+                        | _::_ => HMAC_DRBG_update HMAC additional_input key v
+                      end in
+      let (v, temp) := HMAC_DRBG_generate_helper_Z HMAC key v requested_number_of_bytes in
+      let returned_bits := firstn (Z.to_nat requested_number_of_bytes) temp in
+      let (key, v) := HMAC_DRBG_update HMAC additional_input key v in
+      let reseed_counter := reseed_counter + 1 in
+      generate_algorithm_success returned_bits (v, key, reseed_counter)
+  end.
