specs/DRBG_generate_function.v
@@ -17,30 +17,31 @@ Fixpoint DRBG_generate_function_helper (generate_algorithm: DRBG_working_state -
   match result with
     | ENTROPY.error e s => ENTROPY.error e s
     | ENTROPY.success (state_handle, additional_input) entropy_stream =>
-      let '(working_state, security_strength, prediction_resistance_flag) := state_handle in
-      match generate_algorithm working_state requested_number_of_bytes additional_input with
-        | generate_algorithm_reseed_required =>
-          match count with
-            | O => ENTROPY.error ENTROPY.generic_error entropy_stream (* impossible *)
-            | S count' => DRBG_generate_function_helper generate_algorithm reseed_function entropy_stream state_handle requested_number_of_bytes prediction_resistance_request additional_input true count'
-          end
-        | generate_algorithm_success x y => ENTROPY.success (x, y) entropy_stream
+      match state_handle with (working_state, security_strength, prediction_resistance_flag) =>
+        match generate_algorithm working_state requested_number_of_bytes additional_input with
+          | generate_algorithm_reseed_required =>
+            match count with
+              | O => ENTROPY.error ENTROPY.generic_error entropy_stream (* impossible *)
+              | S count' => DRBG_generate_function_helper generate_algorithm reseed_function entropy_stream state_handle requested_number_of_bytes prediction_resistance_request additional_input true count'
+            end
+          | generate_algorithm_success x y => ENTROPY.success (x, y) entropy_stream
+        end
       end
     end.
 
 Definition DRBG_generate_function (generate_algorithm: Z -> DRBG_working_state -> Z -> list Z -> DRBG_generate_algorithm_result) (reseed_function: ENTROPY.stream -> DRBG_state_handle -> bool -> list Z -> ENTROPY.result DRBG_state_handle) (reseed_interval: Z) (max_number_of_bytes_per_request: Z) (max_additional_input_length: Z) (entropy_stream: ENTROPY.stream) (state_handle: DRBG_state_handle) (requested_number_of_bytes requested_security_strength: Z) (prediction_resistance_request: bool) (additional_input: list Z): ENTROPY.result (list Z * DRBG_state_handle) :=
-  let '(working_state, security_strength, prediction_resistance_flag) := state_handle in
-  if Z.gtb requested_number_of_bytes max_number_of_bytes_per_request then ENTROPY.error ENTROPY.generic_error entropy_stream
-  else
-    if Z.gtb requested_security_strength security_strength then ENTROPY.error ENTROPY.generic_error entropy_stream
+  match state_handle with (working_state, security_strength, prediction_resistance_flag) =>
+    if Z.gtb requested_number_of_bytes max_number_of_bytes_per_request then ENTROPY.error ENTROPY.generic_error entropy_stream
     else
-      if Z.gtb (Zlength additional_input) max_additional_input_length then ENTROPY.error ENTROPY.generic_error entropy_stream
+      if Z.gtb requested_security_strength security_strength then ENTROPY.error ENTROPY.generic_error entropy_stream
       else
-        if prediction_resistance_request && (negb prediction_resistance_flag) then ENTROPY.error ENTROPY.generic_error entropy_stream
+        if Z.gtb (Zlength additional_input) max_additional_input_length then ENTROPY.error ENTROPY.generic_error entropy_stream
         else
-          match DRBG_generate_function_helper (generate_algorithm reseed_interval) reseed_function entropy_stream state_handle requested_number_of_bytes prediction_resistance_request additional_input prediction_resistance_request 1%nat with
-            | ENTROPY.error e s => ENTROPY.error e s
-                                                 | ENTROPY.success (output, new_working_state) entropy_stream =>
-                                                   ENTROPY.success (output, (new_working_state, security_strength, prediction_resistance_flag)) entropy_stream
-          end.
-
+          if prediction_resistance_request && (negb prediction_resistance_flag) then ENTROPY.error ENTROPY.generic_error entropy_stream
+          else
+            match DRBG_generate_function_helper (generate_algorithm reseed_interval) reseed_function entropy_stream state_handle requested_number_of_bytes prediction_resistance_request additional_input prediction_resistance_request 1%nat with
+              | ENTROPY.error e s => ENTROPY.error e s
+                                                   | ENTROPY.success (output, new_working_state) entropy_stream =>
+                                                     ENTROPY.success (output, (new_working_state, security_strength, prediction_resistance_flag)) entropy_stream
+            end
+  end.
