specs/DRBG_reseed_function.v
@@ -5,7 +5,7 @@ Require Import DRBG_working_state.
 Require Import entropy.
 
 Definition DRBG_reseed_function (reseed_algorithm: DRBG_working_state -> list Z -> list Z -> DRBG_working_state) (min_entropy_length max_entropy_length: Z) (max_additional_input_length: Z) (entropy_stream: ENTROPY.stream) (state_handle: DRBG_state_handle) (prediction_resistance_request: bool) (additional_input: list Z): ENTROPY.result DRBG_state_handle :=
-  let '(working_state, security_strength, prediction_resistance_flag) := state_handle in
+  match state_handle with (working_state, security_strength, prediction_resistance_flag) =>
   if prediction_resistance_request && (negb prediction_resistance_flag) then ENTROPY.error ENTROPY.generic_error entropy_stream
   else
     if Z.gtb (Zlength additional_input) max_additional_input_length then ENTROPY.error ENTROPY.generic_error entropy_stream
@@ -15,4 +15,6 @@ Definition DRBG_reseed_function (reseed_algorithm: DRBG_working_state -> list Z 
         | ENTROPY.success entropy_input entropy_stream =>
           let new_working_state := reseed_algorithm working_state entropy_input additional_input in
           ENTROPY.success (new_working_state, security_strength, prediction_resistance_flag) entropy_stream
-      end.
+      end
+  end.
+
